

Question Bank

Q1.

Question Bank

PAGE No.	
DATE	/ /

1) $[x^2 - 4xy - 2y^2] dx + [y^2 - 4xy - 2x^2] dy = 0$

$M dx + N dy = 0$

$M = x^2 - 4xy - 2y^2$ $N = y^2 - 4xy - 2x^2$

$\frac{\partial M}{\partial y} = -4x - 4y$ $\frac{\partial N}{\partial x} = -4y - 4x$

$\frac{\partial M}{\partial y} = \frac{\partial N}{\partial x}$

The eqⁿ is exact.

The solⁿ is

$\int M dx + \int N dy = c$

~~$\int (x^2 - 4xy - 2y^2) dx + \int (y^2 - 4xy - 2x^2) dy = 0$~~

~~$\frac{x^3}{3} - \frac{4x^2y}{2} - 2xy^2 + \frac{y^3}{3} - \frac{4xy^2}{2} - 2x^2y = 0$~~

$\frac{x^3}{3} = \int (x^2 - 4xy - 4y) dx + \int y^2 dy = c$

$\frac{x^3}{3} = \frac{4x^2y}{2} - 2xy^2 + \frac{y^3}{3} = c$

$\frac{x^3}{3} - 2x^2y - 2xy^2 + \frac{y^3}{3} = c$

$x^3 - 6x^2y - 6xy^2 + y^3 = 3c$

Q2.

$$2) [x\sqrt{x^2+y^2} - y] dx + [y\sqrt{x^2+y^2} - x] dy = 0$$

$$M = x\sqrt{x^2+y^2} - y \quad N = y\sqrt{x^2+y^2} - x$$

$$\frac{\partial M}{\partial y} = \frac{x \cdot 2y}{2\sqrt{x^2+y^2}} - 1 \quad \frac{\partial N}{\partial x} = \frac{2xy}{2\sqrt{x^2+y^2}} - 1$$

$$\boxed{\frac{\partial M}{\partial y} = \frac{\partial N}{\partial x}}$$

This eqⁿ is exact

The solⁿ is

$$\int M dx + \int N dy = c$$

$$\int (x\sqrt{x^2+y^2} - y) dx + \int 0 dy = c$$

$$\text{Put } x^2+y^2 = t$$

$$2x = \frac{dt}{dx}$$

$$x dx = \frac{dt}{2}$$

$$\int \frac{t}{2} \frac{dt}{2} - \int y dx = c$$

$$\frac{1}{2} \frac{t^2}{2} = xy = c$$

$$\boxed{\frac{1}{3} (x^2+y^2)^{3/2} - xy = c}$$

$$\boxed{(x^2+y^2)^{3/2} - 3xy = 3c}$$

Q3.

g) $[1 + \log(xy)] dx + [1 + \frac{x}{y}] dy = 0$

$$M = 1 + \log(xy) \quad N = 1 + \frac{x}{y}$$

$$\frac{\partial M}{\partial y} = \frac{1}{xy} x$$

$$\frac{\partial N}{\partial x} = \frac{1}{y}$$

$$\frac{\partial M}{\partial y} = \frac{1}{y}$$

$$\boxed{\frac{\partial M}{\partial y} = \frac{\partial N}{\partial x}}$$

The eqn exact

The soln is

$$\int M dx + \int N dy = c$$

$$\int [1 + \log(xy)] dx + \int 1 dy = c$$

$$x + \int \log(xy) dx + y = c$$

$$x + \left[\log(xy) \int 1 dx - \int \frac{d}{dx} \log xy \int 1 dx dx \right] + y = c$$

$$x + \left[x \log xy - \int \frac{1}{xy} y x dx \right] + y = c$$

$$x + x \log xy - \int 1 dx + y = c$$

$$x + x \log xy - x + y = c$$

$$\boxed{x \log xy + y = c}$$

Q4.

9) $(x^3y^4 + x^2y^3 + xy^2 + y)dx + (x^4y^3 - x^3y^2 - x^2y + x)dy = 0$

$$M = x^3y^4 + x^2y^3 + xy^2 + y$$

$$\frac{\partial M}{\partial y} = 4x^3y^3 + 3x^2y^2 + 2xy + 1$$

$$N = x^4y^3 - x^3y^2 - x^2y + x$$

$$\frac{\partial N}{\partial x} = 4x^3y^3 - 3x^2y^2 - 2xy + 1$$

$$\left[\frac{\partial M}{\partial y} \neq \frac{\partial N}{\partial x} \right]$$

The eqn is not exact.

$$Mx - Ny = x(x^3y^4 + x^2y^3 + xy^2 + y) - y(x^4y^3 - x^3y^2 - x^2y + x)$$

$$= x^4y^4 + x^3y^3 + x^2y^2 + xy - x^4y^4 + x^3y^3 + x^2y^2 - xy$$

$$Mx - Ny = 2x^3y^3 + 2x^2y^2$$

$$IF = \frac{1}{2x^3y^3(xy+1)} \quad IF = \frac{1}{Mx - Ny}$$

$$IF = \frac{1}{2x^3y^3(xy+1)}$$

multiply eqn ① by IF

$$\frac{(x^3y^4 + x^2y^3 + xy^2 + y)}{2x^3y^3(xy+1)} dx + \frac{(x^4y^3 - x^3y^2 - x^2y + x)}{2x^3y^3(xy+1)} dy = 0$$

$$\frac{x^2y^3(xy+1) + y(xy+1)}{2x^3y^3(xy+1)} dx + \frac{(x^3y^3(xy+1) - x(xy+1))}{2x^3y^3(xy+1)} dy = 0$$

$$\frac{(xy+1)(x^2y^3+y)}{2x^3y^3(xy+1)} dx + \frac{(xy-1)(x^3y^2-x)}{2x^3y^3(xy+1)} dy = 0$$

$$\frac{y(x^2y^3+y)}{2x^3y^3} dx + \frac{(xy-1)x(x^2y^2-1)}{2x^3y^3(xy+1)} dy = 0$$

$$\frac{y(x^2y^2+1)}{2x^3y^3} dx + \frac{x(xy-1)(xy-1)(xy+1)}{2x^3y^3(xy+1)} dy = 0$$

$$\frac{(x^2y^3+1)}{2x^2y} dx + \frac{(xy-1)^2}{2xy^2} dy = 0$$

$$M' = \frac{x^2y^3+1}{2x^2y}$$

$$N' = \frac{(xy-1)^2}{2xy^2}$$

$$M' = \frac{x^2y^3}{2x^2y} + \frac{1}{2x^2y}$$

$$N' = \frac{x^2y^3}{2xy^2} - \frac{2xy}{2xy^2} + \frac{1}{2xy^2}$$

$$M' = \frac{y}{2} + \frac{1}{2x^2y}$$

$$N' = \frac{x}{2} - \frac{1}{y} + \frac{1}{2xy^2}$$

$$\frac{\partial M'}{\partial y} = \frac{1}{2} - \frac{1}{2x^2y^2}$$

$$\frac{\partial N'}{\partial x} = \frac{1}{2} - \frac{1}{2x^2y}$$

$$\boxed{\frac{\partial M'}{\partial y} = \frac{\partial N'}{\partial x}}$$

The eqⁿ is exact

The solⁿ is

$$\int M' dx + \int N' dy = C$$

$$\int \left(\frac{y}{2} + \frac{1}{2x^2y} \right) dx + \int -\frac{1}{y} dy = C$$

$$\boxed{\frac{xy}{2} - \frac{1}{2xy} - \log y = C}$$

$$\boxed{xy - \frac{1}{xy} - 2 \log y = 2C}$$

Q5.

10) $(2xy^4e^y + 2xy^3 + 4)dx + (x^2y^4e^y - x^2y^2 - 3x)dy = 0$ — (1)

$M = 2xy^4e^y + 2xy^3 + 4$ $N = x^2y^4e^y - x^2y^2 - 3x$

$\frac{\partial M}{\partial y} = 2x(4y^3e^y + y^3 + 3y^2) + 6xy^2 + 1$

$\frac{\partial N}{\partial x} = 2xy^4e^y - 2xy^2 - 3$

$\left[\frac{\partial M}{\partial y} \neq \frac{\partial N}{\partial x} \right]$

The eq is not exact

$Mx - Ny = x(2xy^4e^y + 2xy^3 + 4) - y(x^2y^4e^y - x^2y^2 - 3x)$

$= 2x^2y^4e^y + 2x^2y^3 + 4xy - x^3y^4e^y + x^3y^2 + 3xy$

$\frac{\partial M}{\partial y} - \frac{\partial N}{\partial x} = 2xy^4e^y + 8xy^3e^y + 6xy^2 + 1 - 2$

$\frac{\partial M}{\partial y} - \frac{\partial N}{\partial x} = \frac{2xy^4e^y - 2xy^2 - 3 - 2xy^4e^y + 8xy^3e^y}{2xy^4e^y + 2xy^3 + 4}$

$= \frac{-8xy^2 - 8xy^3e^y - 2}{2xy^4e^y + 2xy^3 + 4}$

$$\frac{\frac{\partial M}{\partial y} - \frac{\partial N}{\partial x}}{M} = \frac{-4(2xy^3e^y + 2xy^2 + 1)}{4(2xy^3e^y + 2xy^2 + 1)}$$

$$f(y) = -\frac{4}{y}$$

$$\int f(y) dy$$

$$I.P = e$$

$$= 4 \int \frac{1}{y} dy$$

$$= e$$

$$= 4 \log y$$

$$= e$$

$$= e^{\log \frac{1}{y^4}}$$

$$I.P = \frac{1}{y^4}$$

multiply eqn (1) by I.P

$$\left(\frac{2xy^4e^y}{y^4} + \frac{2xy^2}{y^4} + \frac{1}{y^4} \right) dx + \left(\frac{x^2y^4e^y}{y^4} - \frac{x^2y^2}{y^4} - \frac{3x}{y^4} \right) dy$$

$$\left(2xe^y + \frac{2x}{y} + \frac{1}{y^3} \right) dx + \left(x^2e^y - \frac{x^2}{y^2} - \frac{3x}{y^4} \right) dy$$

$$M' = 2xe^y + \frac{2x}{y} + \frac{1}{y^3} \quad N' = x^2e^y - \frac{x^2}{y^2} - \frac{3x}{y^4}$$

$$\frac{\partial M'}{\partial y} = 2xe^y - \frac{2x}{y^2} - \frac{3}{y^4} \quad \frac{\partial N'}{\partial x} = 2xe^y - \frac{2x}{y^2} - \frac{3}{y^4}$$

$$\frac{\partial M'}{\partial y} = \frac{\partial N'}{\partial x}$$

The eqⁿ is exact.

The solⁿ is

$$\int M dx + \int N dy = C$$

$$\int \left(2xe^y + \frac{2x}{y} + \frac{1}{y^3} \right) dx + \int 0 dy = C$$

$$\frac{x^2 e^y}{2} + \frac{x^2}{2y} + \frac{x}{y^3} = C$$

$$\boxed{\frac{x^2 e^y}{2} + \frac{x^2}{2y} + \frac{x}{y^3} = C}$$

Q6. A

⑤

(A) $(1+x^2) \frac{dy}{dx} + 2xy - 4x^2 = 0$

$$(1+x^2) dy = -(2xy - 4x^2) dx$$

$$(2xy - 4x^2) dx + (1+x^2) dy = 0$$

$$M = 2xy - 4x^2 \quad N = 1 + x^2$$

$$\frac{\partial M}{\partial y} = 2x$$

$$\frac{\partial N}{\partial x} = 2x$$

$$\boxed{\frac{\partial M}{\partial y} = \frac{\partial N}{\partial x}}$$

The eqn is exact

The solⁿ is

$$\int M dx + \int N dy = c$$

$$\int (2xy - 4x^2) dx + \int 1 dy = c$$

$$\frac{x^2 y}{x} - \frac{4x^3}{3} + y = c$$

$$\boxed{x^2 y - \frac{4x^3}{3} + y = c}$$

B

$$(B) (1+y^2) dx = (\tan^{-1} y - x) dy$$

$$(1+y^2) dx + -(\tan^{-1} y - x) dy$$

$$M = 1+y^2 \quad N = -\tan^{-1} y + x$$

$$\frac{\partial M}{\partial y} = 2y \quad \frac{\partial N}{\partial x} = 1$$

$$\boxed{\frac{\partial M}{\partial y} \neq \frac{\partial N}{\partial x}}$$

This eqⁿ is not exact

$$\frac{dx}{dy} = \frac{\tan^{-1} y - x}{(1+y^2)}$$

$$\frac{dx}{dy} = \frac{\tan^{-1} y}{1+y^2} - \frac{x}{1+y^2}$$

$$\frac{dx}{dy} + \frac{x}{1+y^2} = \frac{\tan^{-1} y}{1+y^2}$$

$$\frac{dx}{dy} + P x = Q$$

This is linear diff. eqⁿ

$$I.P. = e^{\int P dy}$$

$$P = \frac{1}{1+y^2}$$

$$Q = \frac{\tan^{-1} y}{1+y^2}$$

$$\text{I.P} = \int \frac{1}{1+y^2} dy$$

$$\text{I.F} = e^{\tan^{-1}y}$$

The solⁿ is

$$\text{I.P} = \int q \text{ I.F} dy + c$$

$$x e^{\tan^{-1}y} = \int \frac{\tan^{-1}y}{1+y^2} e^{\tan^{-1}y} dy + c$$

$$\text{put } \tan^{-1}y = t$$

$$\frac{1}{1+y^2} dy = dt$$

$$x e^t = \int t e^t dt + c$$

$$x e^t = t \int e^t dt - \int \frac{dt}{dt} \int e^t dt + c$$

$$x e^t = t e^t - \int e^t dt + c$$

$$= t e^t - e^t + c$$

$$x e^t = e^t (t-1) + c$$

$$\boxed{x e^{\tan^{-1}y} = e^{\tan^{-1}y} (\tan^{-1}y - 1) + c}$$

Q7. A

PAGE No.	
DATE	/ /

$$(3) (A) \frac{dy}{dx} = e^{x-y} (e^x - e^y)$$

$$\frac{dy}{dx} = e^{2x-y} - e^{x-y+y}$$

$$= e^{2x} \cdot e^{-y} - e^x$$

$$\frac{dy}{dx} + e^x = \frac{e^{2x}}{e^y}$$

$$e^y \frac{dy}{dx} + e^x e^y = e^{2x}$$

put $e^y = v$
diff w.r.t. x

$$e^y \frac{dy}{dx} = \frac{dv}{dx}$$

$$\frac{dv}{dx} + e^x v = e^{2x}$$

This is linear diff. eqⁿ

$$P = e^x \quad Q = e^{2x}$$

$$\text{I.F} = e^{\int P dx} = e^{\int e^x dx} = e^{e^x}$$

$$\boxed{\text{I.F} = e^{e^x}}$$

The soln is

$$\forall \text{ I.P} = \int \text{I.P} \phi \, dx + c$$

$$e^y e^x = \int e^x e^{2x} \, dx + c$$

$$= \int e^x e^x e^x \, dx + c$$

$$\text{put } e^x = t$$

diff. w.r.t. x

$$e^x \, dx = dt$$

$$e^y e^t = \int e^t \cdot t \, dt + c$$

$$= t \int e^t - \int \frac{dt}{dt} \int e^t \, dt + c$$

$$= t e^t - \int e^t \, dt + c$$

$$= t e^t - e^t + c$$

$$e^y e^t = e^t (t - 1) + c$$

$$\boxed{e^y e^x = e^x (e^x - 1) + c}$$

B

PAGE No.	
DATE	/ /

$$\textcircled{B} \quad x \frac{dy}{dx} + y = x^3 y^6$$

$$\frac{x}{y^6} \frac{dy}{dx} + \frac{y}{dy^6} = x^3$$

$$\frac{1}{y^6} \frac{dy}{dx} + \frac{1}{x y^5} = x^2$$

$$\text{put } \frac{1}{y^5} = v$$

diff. w.r.t. x

$$\frac{1}{y^6} \frac{dy}{dx} - \frac{5}{y^6} \frac{dy}{dx} = \frac{dv}{dx}$$

$$\frac{1}{y^6} \frac{dy}{dx} = \frac{-1}{5} \frac{dv}{dx}$$

$$-\frac{1}{5} \frac{dv}{dx} + \frac{1}{x} v = x^2$$

$$\frac{dv}{dx} - \frac{5}{x} v = -5x^2$$

This is linear diff. eqⁿ

$$\frac{dv}{dx} + p v = q$$

$$p = -\frac{5}{x} \quad q = -5x^2$$

$$\text{I.F.} = e^{\int p dx}$$

$$\begin{aligned} \text{I.F} &= e^{\int \frac{1}{x} dx} \\ &= e^{-5 \log x} \\ &= e^{\log \frac{1}{x^5}} \end{aligned}$$

$$\boxed{\text{I.F} = \frac{1}{x^5}}$$

The solⁿ is

$$\text{V.I.F} = \int \text{I.F} \cdot \phi \, dx + C$$

$$\frac{1}{y^5} \frac{1}{x^5} = \int \frac{1}{x^5} (-5x^4) \, dx + C$$

$$\frac{1}{y^5 x^5} = -5 \int \frac{1}{x^3} \, dx + C$$

$$\frac{1}{y^5 x^5} = -5 \left(\frac{-1}{2x^2} \right) + C$$

$$\boxed{\frac{1}{y^5 x^5} = \frac{5}{2x^2} + C}$$

8. A

DATE / /

12) (A) $(D^2 - 6D + 9)Y = 0$

Auxillary Equation is

$$D^2 - 6D + 9 = 0$$

$$D = 3, 3$$

$$C.F = e^{3x} (C_1 x + C_2)$$

$$Y = C.F$$

$$Y = e^{3x} (C_1 x + C_2)$$

B

13) (A) $(D^4 + k^4)Y = 0$

Auxillary eqⁿ is

$$D^4 + k^4 = 0$$

$$D^4 + k^4 + 2D^2 k^2 - 2D^2 k^2 = 0$$

$$(D^2 + k^2)^2 - (\sqrt{2} Dk)^2 = 0$$

$$(D^2 + k^2 - \sqrt{2} Dk)(D^2 + k^2 + \sqrt{2} Dk) = 0$$

$$D^2 + k^2 - \sqrt{2} Dk = 0$$

$$D^2 + k^2 + \sqrt{2} Dk = 0$$

$$D^2 - \sqrt{2}DK + K^2 = 0$$

$$aD^2 + Bx + C = 0$$

$$a = 1, B = -\sqrt{2}K, C = K^2$$

$$D = \frac{-b \pm \sqrt{b^2 - 4ac}}{2a}$$

$$D = \frac{\sqrt{2}K \pm \sqrt{2K^2 - 4K^2}}{2a}$$

$$D = \frac{\sqrt{2}K \pm \sqrt{2K^2}}{2a}$$

$$D = \frac{\sqrt{2}K \pm i\sqrt{2}K}{2}$$

$$D = \frac{\sqrt{2}(K \pm iK)}{2}$$

$$D = \frac{K \pm iK}{\sqrt{2}}$$

$$D = \frac{K}{\sqrt{2}} \pm \frac{K}{\sqrt{2}}$$

$$\alpha = \frac{K}{\sqrt{2}} \quad \beta = \frac{K}{\sqrt{2}}$$

$$D^2 + \sqrt{2}DK + K^2 = 0$$

$$D = \frac{-K \pm iK}{\sqrt{2}}$$

$$D = \frac{-k}{\sqrt{2}} \pm \frac{ik}{\sqrt{2}}$$

$$\alpha = -\frac{k}{\sqrt{2}} \quad \beta = \frac{k}{\sqrt{2}}$$

The solⁿ is

$$y = \text{---}$$

$$y = e^{\frac{kx}{\sqrt{2}}} \left[C_1 \cos \frac{k}{2} x + C_2 \sin \frac{k}{2} x \right] + e^{-\frac{kx}{\sqrt{2}}} \left[C_3 \cos \frac{k}{2} x + C_4 \sin \frac{k}{2} x \right]$$

C

$$(B) (D-1)^2 (D^2+1) y = 0$$

Auxillary eqⁿ is

$$(D-1)^2 = 0$$

$$(D^2+1) = 0$$

$$D^2 - 2D + 1 = 0$$

$$D = 1, 1$$

$$D^2 + 1 = 0$$

$$D^2 = -1$$

$$D = \pm i$$

$$y = e^x (C_1 x + C_2) + e^{0x} (C_3 \cos x + C_4 \sin x)$$

$$y = e^x (C_1 x + C_2) + C_3 \cos x + C_4 \sin x$$

Q9. A

(14) $(D^2 + 2)y = e^x - \cos 2x$

(A)

$$AE: D^2 + 2 = 0$$

$$D^2 = -2$$

$$D = \pm i\sqrt{2}$$

$$C.F = e^{0x} (C_1 \cos \sqrt{2}x + C_2 \sin \sqrt{2}x)$$

$$C.P = C_1 \cos \sqrt{2}x + C_2 \sin \sqrt{2}x$$

$$P.I = \frac{1}{f(D)} \times (e^x - \cos 2x)$$

$$= \frac{1}{D^2 + 2} (e^x - \cos 2x)$$

$$= \frac{e^x}{D^2 + 2} - \frac{\cos 2x}{D^2 + 2}$$

$$= \frac{e^x}{1 + 2} - \frac{\cos 2x}{-(2)^2 + 2}$$

$$P.I = \frac{e^x}{3} + \frac{\cos 2x}{6}$$

The solⁿ is

$$y = C.F + P.I$$

$$y = C_1 \cos \sqrt{2}x + C_2 \sin \sqrt{2}x + \frac{e^x}{3} + \frac{\cos 2x}{6}$$

B

PAGE No.	
DATE	/ /

$$(B) (D^3 - 2D^2 - 5D + 6) y = e^{3x} + 8$$

Auxiliary eqⁿ is

$$D^3 - 2D^2 - 5D + 6 = 0$$

$$D = -2, 3, 1$$

$$C.F. = C_1 e^{-2x} + C_2 e^{3x} + C_3 e^x$$

$$P.I. = \frac{1}{D^3 - 2D^2 - 5D + 6} \times (e^{3x} + 8)$$

$$P.I. = \frac{e^{3x}}{D^3 - 2D^2 - 5D + 6} + \frac{8e^{0x}}{D^3 - 2D^2 - 5D + 6}$$

$$P.I. = \frac{2e^{3x}}{3D^2 - 4D - 5} + \frac{8}{(0)^3 - 2(0)^2 - 5(0) + 6}$$

$$= \frac{x e^{3x}}{2(3)^2 - 4(3) - 5} + \frac{8}{6}$$

$$P.I. = \frac{2e^{3x}}{10} + \frac{4}{3}$$

Q10. A

(15) $\frac{d^2y}{dx^2} - 4\frac{dy}{dx} + 4y = e^x + \cos 2x$
 (A)

$$\cancel{D^2 - 4D} D^2y - 4Dy + 4y = e^x + \cos 2x$$

$$(D^2 - 4D + 4)y = e^x + \cos 2x$$

Auxiliary eqⁿ is

$$D^2 - 4D + 4 = 0$$

$$D = 2, 2$$

$$C.F. = e^{2x} (C_1x + C_2)$$

$$P.I. = \frac{1}{f(D)} e^x + \cos 2x$$

$$P.I. = \frac{e^x}{D^2 - 4D + 4} + \frac{\cos 2x}{D^2 - 4D + 4}$$

$$P.I. = \frac{e^x}{(1)^2 - 4(1) + 4} + \frac{\cos 2x}{-(2)^2 - 4(2) + 4}$$

$$P.I. = \frac{e^x}{1 - 4 + 4} + \frac{\cos 2x}{-4 - 4 + 4}$$

$$P.I. = \frac{e^x}{1} + \frac{\cos 2x}{-4}$$

$$P.I. = e^x - \frac{1}{4} \cos 2x$$

$$P.I = e^x - \frac{1}{4} \int \cos 2x \, dx$$

$$P.I = e^x - \frac{1}{4} \left(\frac{\sin 2x}{2} \right)$$

$$P.I = e^x - \frac{\sin 2x}{8}$$

$$y = C.F + P.I$$

$$y = e^{2x} (C_1 x + C_2) + e^x - \frac{\sin 2x}{8}$$

B

$$(B) \quad (D^2 + 4D + 4) y = \cosh 2x$$

$$A.E = D^2 + 4D + 4 = 0$$

$$D = -2, -2$$

$$C.F = e^{-2x} (C_1 x + C_2)$$

$$P.I = \frac{1}{D^2 + 4D + 4} \times \cosh 2x$$

$$= \frac{1}{D^2 + 4D + 4} \times \left(\frac{e^{2x} + e^{-2x}}{2} \right)$$

$$= \frac{1}{2} \left[\frac{e^{2x}}{D^2 + 4D + 4} + \frac{e^{-2x}}{D^2 + 4D + 4} \right]$$

$$= \frac{1}{2} \left[\frac{e^{2x}}{(2)^2 + 4(2) + 4} + \frac{x e^{-2x}}{2D + 4} \right]$$

$$\frac{1}{2} \left[\frac{e^{2x}}{16} + \frac{x^2 e^{-2x}}{2} \right]$$

$$P.I = \frac{e^{2x}}{32} + \frac{x^2 e^{-2x}}{4}$$

$$y = C.F \neq P.I$$

$$y = e^{2x}(C_1 x + C_2) + \frac{e^{2x}}{32} + \frac{x^2 e^{-2x}}{4}$$

Q11. i)

(17) Evaluate

$$\textcircled{1} \int_0^{\infty} e^{-h^2 x^2} dx$$

$$\text{Put } h^2 x^2 = t$$

$$x^2 = \frac{t}{h^2}$$

$$x = \frac{\sqrt{t}}{h}$$

$$dx = \frac{1}{2h} \frac{1}{\sqrt{t}} dt$$

$$= \int_0^{\infty} e^{-t} \frac{1}{2h} \frac{1}{\sqrt{t}} dt$$

$$= \frac{1}{2h} \int_0^{\infty} e^{-t} t^{-\frac{1}{2}} dt$$

$$= \frac{1}{2h} \int_0^{\infty} e^{-t} t^{-\frac{1}{2}+1-1} dt$$

$$\int_0^{\infty} e^{-x} x^{n-1} dx = \Gamma(n)$$

$$= \frac{1}{2h} \Gamma\left[-\frac{1}{2}+1\right]$$

$$= \frac{1}{2h} \Gamma\left[\frac{1}{2}\right]$$

$$= \frac{1}{2h} \sqrt{\pi}$$

ii)

$$\begin{aligned} \textcircled{a} \quad & \int_0^{\infty} e^{-x} x^{3/2} dx \\ &= \int_0^{\infty} e^{-x} x^{3/2+1-1} dx \\ &= \int_0^{\infty} e^{-x} x^{5/2-1} dx \\ & \int_0^{\infty} e^{-x} x^{n+1} dx = \Gamma(n) \\ &= \Gamma\left(\frac{5}{2}\right) \end{aligned}$$

$$\begin{aligned} &= \left(\frac{5}{2} - 1\right) \Gamma\left(\frac{5}{2} - 1\right) \\ &= \frac{3}{2} \Gamma\left(\frac{3}{2}\right) \\ &= \frac{3}{2} \cdot \frac{1}{2} \Gamma\left(\frac{1}{2}\right) \\ & \boxed{\int_0^{\infty} e^{-x} x^{3/2} dx = \frac{3}{4} \sqrt{\pi}} \end{aligned}$$

iii)

$$\begin{aligned} \textcircled{5} \quad & \int_0^{\infty} x^2 e^{-x^3} dx \\ & \text{put } x^3 = t \\ & x = t^{\frac{1}{3}} \\ & dx = \frac{1}{3} t^{-\frac{2}{3}} dt \\ & = \int_0^{\infty} t^{\frac{1}{3}} e^{-t} \frac{1}{3} t^{-\frac{2}{3}} dt \\ & = \frac{1}{3} \int_0^{\infty} e^{-t} t^{\frac{1}{3} - \frac{2}{3}} dt \\ & = \frac{1}{3} \int_0^{\infty} e^{-t} t^{-\frac{1}{3}} dt \\ & = \frac{1}{3} \int_0^{\infty} e^{-t} t^{-\frac{1}{3} + 1 - 1} dt \\ & = \frac{1}{3} \int_0^{\infty} e^{-t} t^{\frac{3}{3} - 1} dt \\ & = \int_0^{\infty} e^{-x} x^{n-1} dx = \Gamma n \end{aligned}$$

$$\boxed{\int_0^{\infty} x^2 e^{-x^3} dx = \frac{1}{3} \Gamma \frac{3}{3}}$$

iv)

$$\begin{aligned}
 & \textcircled{4} \int_0^{\infty} x^2 e^{-x^4} dx \\
 & \quad x^4 = t \\
 & \quad x = t^{\frac{1}{4}} \\
 & \quad dx = \frac{1}{4} t^{-\frac{3}{4}} dt \\
 & = \int_0^{\infty} t^{\frac{1}{2}} e^{-t} \frac{1}{4} t^{-\frac{3}{4}} dt \\
 & = \frac{1}{4} \int_0^{\infty} e^{-t} t^{\frac{1}{2} - \frac{3}{4}} dt \\
 & = \frac{1}{4} \int_0^{\infty} e^{-t} t^{-\frac{1}{4}} dt \\
 & = \frac{1}{4} \int_0^{\infty} e^{-t} t^{\frac{1}{4} + 1 - 1} dt \\
 & = \frac{1}{4} \int_0^{\infty} e^{-t} t^{\frac{3}{4} - 1} dt
 \end{aligned}$$

PAGE No.	
DATE	/ /

$$\int_0^{\infty} e^{-x} x^{n-1} dx = \Gamma(n)$$

$$\int_0^{\infty} x^2 e^{-x^4} dx = \frac{1}{4} \Gamma\left(\frac{3}{4}\right)$$

V)

PAGE No.	
DATE	/ /

② Evaluate $\int_0^{\infty} x^2 7^{-4x^2} dx$

$$\int_0^{\infty} \frac{x^2}{7^{4x^2}} dx$$

Put $7^{4x^2} = e^t$

$$\log 7^{4x^2} = t$$

$$4x^2 \log 7 = t$$

$$x^2 = \frac{t}{4 \log 7}$$

$$x = \frac{\sqrt{t}}{2\sqrt{\log 7}}$$

$$dx = \frac{1}{2\sqrt{\log 7}} \cdot \frac{1}{2\sqrt{t}} dt$$

$$dx = \frac{t^{-\frac{1}{2}}}{4\sqrt{\log 7}} dt$$

$$I = \int_0^{\infty} \frac{t}{(4 \log 7)^2} \cdot \frac{t^{-\frac{1}{2}}}{4\sqrt{\log 7}} \cdot \frac{1}{e^t} dt$$

$$I = \int_0^{\infty} \frac{e^{-t} t}{4 \log 7} \cdot \frac{t^{\frac{1}{2}}}{4\sqrt{\log 7}} dt$$

$$I = \frac{1}{16 (\log 7)^{3/2}} \int_0^{\infty} e^{-t} t^{\frac{1}{2}+1-1} dt$$

$$I = \frac{1}{16 (\log 7)^{3/2}} \sqrt{\frac{3}{2}}$$

$$= \frac{1}{16 (\log 7)^{3/2}} \cdot \frac{1}{2} \sqrt{\frac{1}{2}}$$

$$I = \frac{\sqrt{\pi}}{32 (\log 7)^{3/2}}$$